Splinter/Betree/ReprBetreeRefinement.i.dfy
@@ -4,12 +4,17 @@
 include "LinkedBetree.i.dfy"
 include "LinkedBetreeRefinement.i.dfy"
 include "ReprBetree.i.dfy"
+include "../../lib/Base/Sets.i.dfy"
 
 module ReprBetreeRefinement
 {
   import opened ReprBetree
   import LinkedBetreeMod
   import LinkedBetreeRefinement
+  import GenericDisk
+  import Sets
+
+  type Ranking = GenericDisk.Ranking
 
   function I(v: Variables) : (out: LinkedBetreeMod.Variables) {
     v.betree
@@ -23,10 +28,15 @@ module ReprBetreeRefinement
   }
 
   predicate Inv(v: Variables) {
+    // Note: ValidRepr and DiskIsTightWrtRepresentation together 
+    // gives us diskView.entries.Keys == v.repr
     && v.WF()
-    && ValidRepr(v)
     && LinkedBetreeRefinement.Inv(v.betree)
+    && ValidRepr(v)                                    // v.repr == Representation
+    && v.betree.linked.DiskIsTightWrtRepresentation()  // diskView == Representation
   }
+
+  //******** PROVE INVARIANTS ********//
 
   lemma InvInit(v: Variables, gcBetree: GCStampedBetree) 
     requires Init(v, gcBetree)
@@ -36,16 +46,54 @@ module ReprBetreeRefinement
     LinkedBetreeRefinement.InitRefines(I(v), gcBetree.I());
   }
 
-  lemma InvNextInternalGrowStep(v: Variables, v': Variables, lbl: TransitionLabel, step: Step)
+  lemma FreshDiskEntriesPreserveReachability(small: LinkedBetree, big: LinkedBetree, addrs: set<Address>, ranking: Ranking) 
+    requires small.Acyclic()
+    requires big.Acyclic()
+    requires big.diskView.entries.Keys == small.diskView.entries.Keys + addrs
+    requires small.diskView.IsSubDisk(big.diskView)
+    requires small.root == big.root
+    requires small.ValidRanking(ranking)
+    requires big.ValidRanking(ranking)
+    ensures small.ReachableAddrsUsingRanking(ranking) == big.ReachableAddrsUsingRanking(ranking)
+    decreases small.GetRank(ranking)
+  {
+    if small.HasRoot() {
+      var numChildren := |small.Root().children|;
+      forall i | 0 <= i < numChildren 
+      ensures small.ChildAtIdx(i).ReachableAddrsUsingRanking(ranking) == big.ChildAtIdx(i).ReachableAddrsUsingRanking(ranking)
+      {
+        LinkedBetreeRefinement.ChildIdxAcyclic(small, i);
+        LinkedBetreeRefinement.ChildIdxAcyclic(big, i);
+        FreshDiskEntriesPreserveReachability(small.ChildAtIdx(i), big.ChildAtIdx(i), addrs, ranking);
+      }
+      var smallSubAddrs := seq(numChildren, i requires 0 <= i < numChildren => small.ChildAtIdx(i).ReachableAddrsUsingRanking(ranking));
+      var bigSubAddrs := seq(numChildren, i requires 0 <= i < numChildren => big.ChildAtIdx(i).ReachableAddrsUsingRanking(ranking));
+      assert smallSubAddrs == bigSubAddrs;  // trigger
+    }
+  }
+
+  lemma GrowStepMaintainsRepr(v: Variables, v': Variables, lbl: TransitionLabel, step: Step)
     requires Inv(v)
     requires NextStep(v, v', lbl, step)
     requires step.InternalGrowStep?
-    ensures Inv(v')
+    requires v'.betree.linked.Acyclic()
+    ensures ValidRepr(v')
   {
-    LinkedBetreeRefinement.InvNextInternalGrowStep(I(v), I(v'), lbl.I(), step.I());
-
-    assume false;
-    assert ValidRepr(v');
+    var linked := v.betree.linked;
+    var linked' := v'.betree.linked;
+    var oldRanking := LinkedBetreeRefinement.BuildTightRanking(linked, linked.TheRanking());
+    var newRanking := LinkedBetreeRefinement.InsertGrowReplacementNewRanking(linked, oldRanking, step.newRootAddr);
+    if v.betree.linked.HasRoot() {
+      LinkedBetreeRefinement.ReachableAddrIgnoresRanking(linked, linked.TheRanking(), oldRanking);
+      LinkedBetreeRefinement.ReachableAddrIgnoresRanking(linked, oldRanking, newRanking);
+      var numChildren := |linked'.Root().children|;
+      var subTreeAddrs := seq(numChildren, i requires 0 <= i < numChildren => linked'.ChildAtIdx(i).ReachableAddrsUsingRanking(newRanking));
+      Sets.UnionSeqOfSetsSoundness(subTreeAddrs);
+      LinkedBetreeRefinement.ChildIdxAcyclic(linked', 0);
+      FreshDiskEntriesPreserveReachability(linked, linked'.ChildAtIdx(0), {step.newRootAddr}, newRanking);
+      LinkedBetreeRefinement.ReachableAddrIgnoresRanking(linked', linked'.TheRanking(), newRanking);
+      assert v'.repr == v'.betree.linked.Representation();
+    }
   }
 
   lemma InvNext(v: Variables, v': Variables, lbl: TransitionLabel) 
@@ -68,8 +116,8 @@ module ReprBetreeRefinement
         assert Inv(v');
       }
       case InternalGrowStep(_) => {
-        // TODO(tony)
-        assume false;
+        LinkedBetreeRefinement.InvNextInternalGrowStep(I(v), I(v'), lbl.I(), step.I());
+        GrowStepMaintainsRepr(v, v', lbl, step);
         assert Inv(v');
       }
       case InternalSplitStep(_, _, _, _) => {
@@ -104,12 +152,16 @@ module ReprBetreeRefinement
     }
   }
 
+
+  //******** PROVE REFINEMENT ********//
+
   lemma InitRefines(v: Variables, gcBetree: GCStampedBetree)
     requires Init(v, gcBetree)
     requires LinkedBetreeRefinement.InvLinkedBetree(gcBetree.I().value)
     ensures Inv(v)
     ensures LinkedBetreeMod.Init(I(v), gcBetree.I())
   {
+    InvInit(v, gcBetree);
     LinkedBetreeRefinement.InitRefines(I(v), gcBetree.I());
   }
 
